---
layout: post
title: Taylor series
author: Zhuyi Xue
tags: statistics
---

Memo for Taylor series, expanding $f(x)$ at $x=a$.

**General form**:

$$
\begin{equation}
f(x) = f(a) + f'(a)(x - a) + \frac{f''(a)}{2!}(x - a)^2 + \frac{f^{(3)}(a)}{3!}(x - a)^3 + \cdots + \frac{f^{(n)}(a)}{n!}(x - a)^n + \cdots
\end{equation}
$$


**Maclaurin series ($a = 0$)**:

$$
\begin{equation}
f(x) = f(0) + f'(0)x + \frac{f''(0)}{2!}x^2 + \frac{f^{(3)}(a)}{3!}x^3 + \cdots + \frac{f^{(n)}(0)}{n!}x^n + \cdots
\end{equation}
$$
